example_iquicksort.v
@@ -73,56 +73,8 @@ End dassert.
 Definition preserves {M : monad} A B (f : A -> M A) (g : A -> B) :=
   forall x, (f x >>= fun y => Ret (y, g y)) = (f x >>= fun y => Ret (y, g x)).
 
-Section more_about_liftM2.
-
-Lemma bind_liftM2 {M : monad} A B C (f : seq A -> seq B -> seq C)
-    (m1 : M (seq A)) (m2 : M (seq B)) n :
-  (forall a b, size (f a b) = size a + size b + n) ->
-  liftM2 f m1 m2 >>= (fun x => Ret (x, size x)) =
-  liftM2 (fun a b => (f a.1 b.1, a.2 + b.2 + n))
-          (m1 >>= (fun x => Ret (x, size x)))
-          (m2 >>= (fun x => Ret (x, size x))).
-Proof.
-move=> hf.
-rewrite /liftM2 !bindA; bind_ext => x1.
-rewrite !bindretf !bindA.
-bind_ext=> x2.
-by rewrite !bindretf /= hf.
-Qed.
-
-Lemma nondetPlus_sub_liftM2 {M : plusMonad} A B C (f : A -> B -> C) (ma : M A) (mb : M B) :
-  nondetPlus_sub ma -> nondetPlus_sub mb ->
-  nondetPlus_sub (liftM2 f ma mb).
-Proof.
-move=> [s1 s1_ma] [s2 s2_mb].
-exists (ndBind s1 (fun a => ndBind s2 (fun b => ndRet (f a b)))).
-by rewrite /= s1_ma s2_mb.
-Qed.
-
-End more_about_liftM2.
-Arguments bind_liftM2 {M A B C} {f} m1 m2 n.
-
 Section more_about_qperm.
 Variable M : plusMonad.
-
-Lemma nondetPlus_sub_splits A (s : seq A) : nondetPlus_sub (splits s : M _).
-Proof.
-elim: s => [|h t ih /=]; first by exists (ndRet ([::], [::])).
-have [syn syn_splits] := ih.
-exists (ndBind syn (fun '(a, b) => ndAlt (ndRet (h :: a, b)) (ndRet (a, h :: b)))).
-rewrite /= syn_splits.
-by bind_ext => -[].
-Qed.
-
-Lemma nondetPlus_sub_tsplits A (s : seq A) : nondetPlus_sub (tsplits s : M _).
-Proof.
-elim: s => [|h t ih]; first by exists (ndRet ([bseq], [bseq])).
-have [syn syn_tsplits] := ih.
-exists (ndBind syn (fun '(a, b) => ndAlt
-    (ndRet ([bseq of h :: a], widen_bseq (leqnSn _) b))
-    (ndRet (widen_bseq (leqnSn _) a, [bseq of h :: b])))).
-by rewrite /= syn_tsplits; bind_ext => -[].
-Qed.
 
 Lemma nondetPlus_sub_qperm A (s : seq A) : nondetPlus_sub (qperm s : M _).
 Proof.
@@ -132,7 +84,7 @@ rewrite qperm_cons.
 rewrite splitsE.
 rewrite fmapE (*TODO: broken ret notation*).
 rewrite bindA.
-have [syn syn_tsplits] := nondetPlus_sub_tsplits t.
+have [syn syn_tsplits] := nondetPlus_sub_tsplits M t.
 have nondetPlus_sub_liftM2_qperm : forall a b : (size t).-bseq A,
   nondetPlus_sub (liftM2 (fun x y => x ++ h :: y) (qperm a) (qperm b : M _)).
   move=> a b; apply nondetPlus_sub_liftM2 => //; apply: ih.
@@ -485,7 +437,7 @@ rewrite qpermE !bindA.
 rewrite !splitsEssplits !fmapE !bindA.
 bind_ext => -[[a b] /= ab].
 rewrite !bindretf.
-rewrite (bind_liftM2 _ _ 1%N); last first.
+rewrite (bind_liftM2_size _ _ 1%N); last first.
   by move=> x y; rewrite size_cat /= addn1 -addnS.
 rewrite {1}/liftM2.
 rewrite ih; last by rewrite (leq_trans _ ns)// ltnS -ab leq_addr.
@@ -547,6 +499,25 @@ by under [in RHS]eq_bind do rewrite bindskipf.
 Qed.
 
 End ssplits.
+
+Section slowsort.
+Variable M : plusMonad.
+Variables (d : unit) (E : orderType d).
+
+Lemma refin_slowsort (p : E) (s : seq E) :
+  Ret (partition p s) >>= (fun '(a, b) =>
+  slowsort a >>= (fun a' => slowsort b >>= (fun b' => Ret (a' ++ p :: b'))))
+  `<=`
+  (slowsort (p :: s) : M _).
+Proof.
+rewrite slowsort_splits.
+apply: refin_trans; first exact/refin_bindr/(partition_spec M p s).
+rewrite bindA; apply: refin_bindl => -[a b].
+rewrite assertE (bindA _ (fun _ => Ret (a, b))) bindretf /= bindA.
+exact: refin_refl.
+Qed.
+
+End slowsort.
 
 Section ssplits_iqsort.
 Variable (d : unit) (E : orderType d) (M : plusArrayMonad E Z_eqType).
@@ -726,20 +697,6 @@ by rewrite (ih (fun s => m (h :: s))) altmm.
 Qed.
 
 End fsplits.
-
-Section more_about_insert.
-Variable (M : plusMonad).
-
-Lemma nondetPlus_sub_insert A (s : seq A) a : nondetPlus_sub (@insert M _ a s).
-Proof.
-elim: s => /= [|h t ih]; first by exists (ndRet [:: a]).
-rewrite insertE /=.
-have [syn synE] := ih.
-exists (ndAlt (ndRet [:: a, h & t]) (ndBind syn (fun x => ndRet (h :: x)))) => /=.
-by rewrite synE fmapE.
-Qed.
-
-End more_about_insert.
 
 Section more_about_perm.
 Variable (M : plusMonad).
@@ -1186,7 +1143,7 @@ have step1 :
      lhs.
      (* l.342 in IQSOrt.agda *)
   rewrite {}/lhs.
-  apply: refin_trans; last by apply: refin_bindr;exact: refin_slowsort.
+  apply: refin_trans; last by apply: refin_bindr; exact: refin_slowsort.
   rewrite bindretf.
   rewrite -qperm_slowsort.
   move Hpxs : (partition p xs) => pxs; case: pxs => [ys zs] in Hpxs *.
